src/Narcissus/Automation/AlignedAutomation.v
@@ -1,0 +1,19 @@
+
+
+Ltac start_synthesizing_encoder :=
+  lazymatch goal with
+  | |- CorrectAlignedEncoderFor ?Invariant ?Spec =>
+    try unfold Spec; try unfold Invariant
+  end;
+  (* Memoize any string constants *)
+  (*pose_string_hyps; *)
+  eexists; simpl; intros.
+
+Ltac align_encoder :=
+    repeat first [
+           apply @CorrectAlignedEncoderForThenC
+         | apply @CorrectAlignedEncoderForDoneC
+         | apply CorrectAlignedEncoderForFormatList
+         | apply CorrectAlignedEncoderForFormatChar; eauto
+         | apply CorrectAlignedEncoderForFormat2Char; eauto
+         | apply CorrectAlignedEncoderForFormatNat].
