src/Narcissus/BinLib.v
@@ -1,0 +1,9 @@
+Require Export
+        Fiat.Narcissus.BinLib.AlignedByteString
+        Fiat.Narcissus.BinLib.AlignWord
+        Fiat.Narcissus.BinLib.AlignedList
+        Fiat.Narcissus.BinLib.AlignedDecoders
+        Fiat.Narcissus.BinLib.AlignedDecodeMonad
+        Fiat.Narcissus.BinLib.AlignedEncodeMonad.
+
+Global Instance ByteStringQueueMonoid : Monoid ByteString := ByteStringQueueMonoid.
